lots of cleanup
- allow ∀ x : X notation for BI ∀
- set precedence levels for pointsto notation
- allow escaping for hl_binder
- implement cons in quicksort example
- change wp lemmas to have generic post

Iris/Iris/HeapLang/Lib/Quicksort.lean
@@ -11,28 +11,25 @@ open BI Iris ProgramLogic
 
 namespace Quicksort
 
-def append : Val := hl_val(
-  rec append f := ref(#false))
+def cons : Val := hl_val% λ x, injr(ref(x))
 
-def cons : Val := hl_val(
-  rec append f := ref(#false))
+def append : Val := hl_val% rec append f := ref(#false)
 
-def partition : Val := hl_val(
-  rec append f := ref(#false))
+def partition : Val := hl_val% rec append f := ref(#false)
 
-def quicksort : Val := hl_val(
+def quicksort : Val := hl_val%
   rec quicksort l :=
     match l with
     | none() => l
     | some(x) =>
-      (let head := fst(x);
-       let tail := snd(x);
+      (let p := !x;
+       let head := fst(p);
+       let tail := snd(p);
        let part := ?partition (head, tail);
        let a := quicksort (fst(part));
        let b := quicksort (snd(part));
        let e := ?cons (head, b);
        ?append (a, e))
-    )
 
 section Predicates
 
@@ -40,7 +37,8 @@ variable [HeapLangGS hlc GF]
 
 def isList (v : Val) : List Int → IProp GF
   | [] => iprop% ⌜v = hl_val(none())⌝
-  | x :: xs => iprop% ∃ tl, ⌜v = hl_val(some((#x, ?tl)))⌝ ∗ isList tl xs
+  | x :: xs => iprop% ∃ l tl, ⌜v = hl_val(some(#(.loc l)))⌝ ∗
+    l ↦ some hl_val((#x, ?tl)) ∗ isList tl xs
 
 end Predicates
 
@@ -49,87 +47,104 @@ section Specs
 variable {GF : BundledGFunctors} [HeapLangGS hlc GF]
 
 theorem cons_spec x l ls Φ :
-  isList (GF:=GF) l ls -∗
-  (∀ v, isList v (x :: ls) -∗ Φ v) -∗
-  WP hl(?cons v((#x, ?l))) {{ Φ }} := by
-    sorry
+    isList (GF:=GF) l ls -∗
+    (∀ v, isList v (x :: ls) -∗ Φ v) -∗
+    WP hl(?cons v((#x, ?l))) {{ Φ }} := by
+  iintro Hl HΦ
+  iapply wp_rec; rfl; simp [Exp.subst, Exp.substStr]
+  imodintro
+  wp_pures
+  wp_bind ref(_)
+  iapply wp_alloc
+  iintro !> %l Hl
+  wp_pures
+  imodintro
+  iapply HΦ
+  rw (occs:=[3]) [isList.eq_def]
+  simp only
+  iexists _, _; iframe
+  itrivial
 
 theorem append_spec l1 ls1 l2 ls2 Φ :
-  isList (GF:=GF) l1 ls1 -∗
-  isList l2 ls2 -∗
-  (∀ v, isList v (ls1 ++ ls2) -∗ Φ v) -∗
-  WP hl(?append v((?l1, ?l2))) {{ Φ }} := by
-    sorry
+    isList (GF:=GF) l1 ls1 -∗
+    isList l2 ls2 -∗
+    (∀ v, isList v (ls1 ++ ls2) -∗ Φ v) -∗
+    WP hl(?append v((?l1, ?l2))) {{ Φ }} := by
+  sorry
 
 theorem partition_spec x l ls Φ :
-  isList (GF:=GF) l ls -∗
-  (∀ l1 l2,
-    isList l1 (ls.filter (· ≤ x)) -∗
-    isList l2 (ls.filter (x < ·)) -∗
-    Φ hl_val((?l1, ?l2))) -∗
-  WP hl(?partition v((#x, ?l))) {{ Φ }} := by
-    sorry
+    isList (GF:=GF) l ls -∗
+    (∀ l1 l2,
+      isList l1 (ls.filter (· ≤ x)) -∗
+      isList l2 (ls.filter (x < ·)) -∗
+      Φ hl_val((?l1, ?l2))) -∗
+    WP hl(?partition v((#x, ?l))) {{ Φ }} := by
+  sorry
 
 -- set_option profiler true in
 theorem quicksort_spec l ls Φ :
-  isList (GF:=GF) l ls -∗
-  (∀ l' ls',
-    isList l' ls' -∗
-    ⌜List.Pairwise LE.le ls'⌝ -∗
-    ⌜List.Perm ls ls'⌝ -∗
-    Φ l') -∗
-  WP hl(?quicksort ?l) {{ Φ }} := by
-    iintro Hl HΦ
-    iloeb as IH generalizing %l %ls %Φ
-    iapply wp_rec; rfl; simp [Exp.subst, Exp.substStr]
+    isList (GF:=GF) l ls -∗
+    (∀ l' ls',
+      isList l' ls' -∗
+      ⌜List.Pairwise LE.le ls'⌝ -∗
+      ⌜List.Perm ls ls'⌝ -∗
+      Φ l') -∗
+    WP hl(?quicksort ?l) {{ Φ }} := by
+  iintro Hl HΦ
+  iloeb as IH generalizing %l %ls %Φ
+  iapply wp_rec; rfl; simp [Exp.subst, Exp.substStr]
+  imodintro
+  rw (occs:=[2]) [isList.eq_def]
+  cases ls with
+  | nil =>
+    simp
+    iclear IH
+    icases Hl with %heq; subst heq
+    wp_pures; simp [Exp.subst]
     imodintro
-    rw (occs:=[2]) [isList.eq_def]
-    cases ls with
-    | nil =>
-      simp
-      iclear IH
-      icases Hl with %heq; subst heq
-      wp_pures; simp [Exp.subst]
-      imodintro
-      iapply HΦ $$ %_ %([])
-      · unfold isList; itrivial
-      · itrivial
-      · itrivial
-    | cons head tail =>
-      simp
-      icases Hl with ⟨%tl, %heq, Hl⟩; subst heq
-      wp_pures; simp [Exp.subst, Exp.substStr]
-      wp_pures; simp [Exp.subst, Exp.substStr]
-      wp_pures; simp [Exp.subst, Exp.substStr]
-      wp_pures
-      wp_bind ?partition _
-      iapply partition_spec $$ [$]
-      iintro %l1 %l2 Hl1 Hl2
-      wp_pures; simp [Exp.subst, Exp.substStr]
-      wp_pures
-      wp_bind ?quicksort _
-      iapply IH $$ [$]
-      iintro %l1' %ls1' Hl1 %_ %_
-      wp_pures; simp [Exp.subst, Exp.substStr]
-      wp_pures
-      wp_bind ?quicksort _
-      iapply IH $$ [$]
-      iintro %l2' %ls2' Hl2 %_ %_
-      wp_pures; simp [Exp.subst, Exp.substStr]
-      wp_pures
-      wp_bind ?cons _
-      iapply cons_spec $$ Hl2
-      iintro %_ _
-      wp_pures; simp [Exp.subst, Exp.substStr]
-      wp_pures
-      iapply append_spec $$ [$] [$]
-      iintro %_ _
-      iapply HΦ $$ [$]
-      · ipureintro
-        have : ls2'.all (head < ·) := by grind
-        grind [List.pairwise_cons]
-      · ipureintro
-        grind [List.filter_append_perm]
+    iapply HΦ $$ %_ %([])
+    · unfold isList; itrivial
+    · itrivial
+    · itrivial
+  | cons head tail =>
+    simp
+    icases Hl with ⟨%l, %tl, %heq, Hpt, Hl⟩; subst heq
+    wp_pures; simp [Exp.subst, Exp.substStr]
+    wp_bind !_
+    iapply wp_load $$ [$]
+    iintro !> Hpt
+    wp_pures; simp [Exp.subst, Exp.substStr]
+    wp_pures; simp [Exp.subst, Exp.substStr]
+    wp_pures; simp [Exp.subst, Exp.substStr]
+    wp_pures
+    wp_bind ?partition _
+    iapply partition_spec $$ [$]
+    iintro %l1 %l2 Hl1 Hl2
+    wp_pures; simp [Exp.subst, Exp.substStr]
+    wp_pures
+    wp_bind ?quicksort _
+    iapply IH $$ [$]
+    iintro %l1' %ls1' Hl1 %_ %_
+    wp_pures; simp [Exp.subst, Exp.substStr]
+    wp_pures
+    wp_bind ?quicksort _
+    iapply IH $$ [$]
+    iintro %l2' %ls2' Hl2 %_ %_
+    wp_pures; simp [Exp.subst, Exp.substStr]
+    wp_pures
+    wp_bind ?cons _
+    iapply cons_spec $$ Hl2
+    iintro %_ _
+    wp_pures; simp [Exp.subst, Exp.substStr]
+    wp_pures
+    iapply append_spec $$ [$] [$]
+    iintro %_ _
+    iapply HΦ $$ [$]
+    · ipureintro
+      have : ls2'.all (head < ·) := by grind
+      grind [List.pairwise_cons]
+    · ipureintro
+      grind [List.filter_append_perm]
 
 
 -- example (l l1 l2 : List Int) x :
